coq-SystemRF-1.1/SystemRF/LemmasNarrowing.v
@@ -1,12 +1,15 @@
 Require Import SystemRF.BasicDefinitions.
 Require Import SystemRF.Names.
 Require Import SystemRF.SystemFTyping.
+Require Import SystemRF.BasicPropsSubstitution.
 Require Import SystemRF.BasicPropsEnvironments.
+Require Import SystemRF.BasicPropsWellFormedness.
 Require Import SystemRF.WellFormedness.
 Require Import SystemRF.Typing.
 Require Import SystemRF.LemmasWeakenWF.
 Require Import SystemRF.LemmasWeakenWFTV.
 Require Import SystemRF.LemmasWellFormedness.
+Require Import SystemRF.SubstitutionLemmaWF.
 Require Import SystemRF.LemmasTyping.
 Require Import SystemRF.LemmasSubtyping.
 Require Import SystemRF.LemmasWeakenTyp.
@@ -19,15 +22,19 @@ Lemma lem_narrow_typ' : ( forall (g'xg : env) (e : expr) (t : type),
             -> unique g -> unique g'
             -> intersect (binds g) (binds g') = empty
             -> ~ (in_env x g) -> ~ (in_env x g') 
-            -> WFtype g s_x k_sx -> WFtype g t_x k_tx -> Subtype g s_x t_x -> WFEnv g
+            -> WFtype g s_x k_sx -> WFtype g t_x k_tx -> Subtype g s_x t_x 
+            -> WFEnv (concatE (Cons x s_x g) g')
             -> Hastype (concatE (Cons x s_x g) g') e t )) /\ (
   forall (g'xg : env) (t : type) (t' : type),
-    Subtype g'xg t t' -> ( forall (g g':env) (x:vname) (s_x t_x:type) (k_sx k_tx:kind),
+    Subtype g'xg t t' -> ( forall (g g':env) (x:vname) (s_x t_x:type) (k_sx k_tx k_t k_t':kind),
       g'xg = concatE (Cons x t_x g) g' 
             -> unique g -> unique g'
             -> intersect (binds g) (binds g') = empty
             -> ~ (in_env x g) -> ~ (in_env x g') 
-            -> WFtype g s_x k_sx -> WFtype g t_x k_tx -> Subtype g s_x t_x -> WFEnv g
+            -> WFtype g s_x k_sx -> WFtype g t_x k_tx -> Subtype g s_x t_x 
+            -> WFEnv (concatE (Cons x s_x g) g')
+            -> WFtype (concatE (Cons x s_x g) g') t  k_t
+            -> WFtype (concatE (Cons x s_x g) g') t' k_t'
             -> Subtype (concatE (Cons x s_x g) g') t t' )).
 Proof. apply ( judgments_mutind 
   (fun (g'xg : env) (e : expr) (t : type) (p_e_t : Hastype g'xg e t) => 
@@ -36,55 +43,64 @@ Proof. apply ( judgments_mutind
             -> unique g -> unique g'
             -> intersect (binds g) (binds g') = empty
             -> ~ (in_env x g) -> ~ (in_env x g') 
-            -> WFtype g s_x k_sx -> WFtype g t_x k_tx -> Subtype g s_x t_x -> WFEnv g
+            -> WFtype g s_x k_sx -> WFtype g t_x k_tx -> Subtype g s_x t_x 
+            -> WFEnv (concatE (Cons x s_x g) g')
             -> Hastype (concatE (Cons x s_x g) g') e t )
   (fun (g'xg : env) (t : type) (t' : type) (p_t_t' : Subtype g'xg t t') => 
-    forall (g g':env) (x:vname) (s_x t_x:type) (k_sx k_tx:kind),
+    forall (g g':env) (x:vname) (s_x t_x:type) (k_sx k_tx k_t k_t':kind),
       g'xg = concatE (Cons x t_x g) g' 
             -> unique g -> unique g'
             -> intersect (binds g) (binds g') = empty
             -> ~ (in_env x g) -> ~ (in_env x g') 
-            -> WFtype g s_x k_sx -> WFtype g t_x k_tx -> Subtype g s_x t_x -> WFEnv g
+            -> WFtype g s_x k_sx -> WFtype g t_x k_tx -> Subtype g s_x t_x 
+            -> WFEnv (concatE (Cons x s_x g) g')
+            -> WFtype (concatE (Cons x s_x g) g') t  k_t
+            -> WFtype (concatE (Cons x s_x g) g') t' k_t'            
             -> Subtype (concatE (Cons x s_x g) g') t t' ));
   intro env; intros; subst env.
   - (* TBC *) apply TBC.
   - (* TIC *) apply TIC.
-  - (* TVar *) apply lem_boundin_concat in b; destruct b;
+  - (* TVar *) 
+    apply lem_truncate_wfenv in H8 as H8'; inversion H8'; subst x1 t0 g0;
+    apply lem_boundin_concat in b; destruct b;
     try destruct H; try destruct H.
     * (* x = x0 *) subst x0; subst t; 
       apply TSub with (self s_x (FV x) k) k;
       try apply TVar; try (apply lem_boundin_concat; left);
+      try apply lem_weaken_many_subtype with k(*_sx*) k(*_tx*);
       try apply lem_selfify_wf;
       try apply lem_weaken_many_wf;
-      try apply lem_weaken_many_subtype;
+      
       try apply lem_exact_subtype with k_sx;
+      try apply lem_weaken_subtype_top with k_sx k_tx;
       try (apply lem_weaken_wf_top; assumption);
-      try apply lem_weaken_subtype_top; try apply WFEBind with k_sx;
-      try rewrite lem_erase_concat;
-      simpl; try rewrite lem_erase_subtype with g s_x t_x; try apply FTVar;
-      try apply lem_boundinF_concatF;
+      try apply WFEBind with k_sx; 
+      try rewrite lem_erase_concat; simpl;
+      try rewrite lem_erase_subtype with g s_x t_x;
+      try apply FTVar; try apply lem_boundinF_concatF;
       try apply intersect_names_add_intro_l; 
-      unfold isLC; simpl; intuition;
+      unfold isLC; simpl;  auto;
       (* WFtype of s_x and t_x, possibly with other kinds *)
       apply lem_weaken_wf_top with g s_x k_sx x s_x in H5 as Hsx;
-      apply lem_weaken_wf_top with g s_x k_sx x t_x in H5 as Hsx';
-      apply lem_weaken_wf_top with g t_x k_tx x t_x in H6 as Htx; trivial;
-      apply lem_narrow_wf_top with g x s_x t_x t_x k_tx in Htx as Htx'; trivial;
+      apply lem_weaken_wf_top with g t_x k_tx x s_x in H6 as Htx; trivial;
       destruct k eqn:K; destruct k_sx eqn:KSX; destruct k_tx eqn:KTX;
       try assumption; try (apply WFKind; assumption);
       (* k_sx = Star but k_tx = Base and k = Base *)
       try ( apply lem_sub_pullback_wftype with t_x;
-            try apply lem_weaken_subtype_top; try apply WFEBind with Star; trivial; reflexivity  );
-      (* k_tx = Star but k = Base *)
-      try ( apply lem_narrow_wf_top with t_x;
-            try apply lem_strengthen_many_wftype_base with g';
-            try apply intersect_names_add_intro_l; simpl; intuition; reflexivity );
+            try apply lem_weaken_subtype_top with Star Base; 
+            try apply WFEBind with Star; trivial; reflexivity  );
+      (* k_tx = Star but k_sx = Base and k = Base *)
+      try ( apply lem_strengthen_many_wftype_base with g';
+            try apply lem_narrow_wf with t_x;
+            try apply intersect_names_add_intro_l; 
+            unfold unique; auto; reflexivity );
       (* k_sx = Star and k_tx = Star but k = Base *)
       try apply lem_sub_pullback_wftype with t_x;
-      try apply lem_narrow_wf_top with t_x;
       try apply lem_strengthen_many_wftype_base with g'; 
-      try apply lem_weaken_subtype_top; try apply WFEBind with Star; 
-      try apply intersect_names_add_intro_l; simpl; intuition.
+      try apply lem_narrow_wf with t_x;
+      try apply lem_weaken_subtype_top with Star Star; 
+      try apply intersect_names_add_intro_l; 
+      unfold unique; auto.
     * (* x in g  *) apply TVar; try apply lem_boundin_concat; simpl;
       try (left; right; apply H); apply lem_narrow_wf with t_x; assumption. 
     * (* x in g' *) apply TVar; try apply lem_boundin_concat; simpl;
@@ -98,8 +114,15 @@ Proof. apply ( judgments_mutind
     assert (Cons y t_x (concatE (Cons x s_x g) g') = concatE (Cons x s_x g) (Cons y t_x g'))
       as Henv by reflexivity; rewrite Henv; 
     apply H with t_x0 k_sx k_tx; 
-    try apply intersect_names_add_intro_r; 
-    try apply not_elem_names_add_intro; simpl; intuition.
+    try apply WFEBind with k_x;
+    try apply lem_narrow_wf with t_x0;
+    try apply intersect_names_add_intro_r;  
+    try apply not_elem_names_add_intro;
+    pose proof (lem_binds_concat (Cons x s_x g) g') as Hc;
+    destruct Hc; try apply not_elem_names_add_intro; trivial;
+    try apply not_elem_subset with (union (binds (Cons x s_x g)) (binds g'));
+    try apply not_elem_union_intro;
+    try apply not_elem_names_add_intro; simpl; auto. 
   - (* TApp *) apply TApp;
     apply H with t_x0 k_sx k_tx || apply H0 with t_x0 k_sx k_tx; trivial.
   - (* TAbsT *) apply TAbsT with (names_add x (union nms (binds (concatE g g')))); intros;
@@ -108,13 +131,18 @@ Proof. apply ( judgments_mutind
     apply not_elem_concat_elim in H11; destruct H11;
     assert (ConsT a' k (concatE (Cons x s_x g) g') = concatE (Cons x s_x g) (ConsT a' k g'))
       as Henv by reflexivity; rewrite Henv; 
-    apply H with t_x k_sx k_tx;
+    apply H with t_x k_sx k_tx; try apply WFEBindT;
     try apply intersect_names_add_intro_r; 
-    try apply not_elem_names_add_intro; simpl; intuition.
+    try apply not_elem_names_add_intro; 
+    pose proof (lem_binds_concat (Cons x s_x g) g') as Hc;
+    destruct Hc; try apply not_elem_names_add_intro; trivial;
+    try apply not_elem_subset with (union (binds (Cons x s_x g)) (binds g'));
+    try apply not_elem_union_intro;
+    try apply not_elem_names_add_intro; simpl; auto.
   - (* TAppT *) apply TAppT with k; try apply H with t_x k_sx k_tx; 
     try apply lem_narrow_wf with t_x; trivial.
   - (* TLet *) apply TLet with t_x k (names_add x (union nms (binds (concatE g g'))));
-    try apply lem_narrow_wf with t_x0; 
+    try apply lem_narrow_wf with t_x0;  
     try apply H with t_x0 k_sx k_tx; trivial; intros;
     apply not_elem_names_add_elim in H1; destruct H1;
     apply not_elem_union_elim in H11; destruct H11;
@@ -122,8 +150,16 @@ Proof. apply ( judgments_mutind
     assert (Cons y t_x (concatE (Cons x s_x g) g') = concatE (Cons x s_x g) (Cons y t_x g'))
       as Henv by reflexivity; rewrite Henv; 
     apply H0 with t_x0 k_sx k_tx; 
+    try apply WFEBind with Star;
+    try apply lem_typing_wf with e_x;
+    try apply H with t_x0 k_sx k_tx; 
     try apply intersect_names_add_intro_r; 
-    try apply not_elem_names_add_intro; simpl; intuition.
+    try apply not_elem_names_add_intro; 
+    pose proof (lem_binds_concat (Cons x s_x g) g') as Hc;
+    destruct Hc; try apply not_elem_names_add_intro; trivial;
+    try apply not_elem_subset with (union (binds (Cons x s_x g)) (binds g'));
+    try apply not_elem_union_intro;
+    try apply not_elem_names_add_intro; simpl; auto.    
   - (* TAnn *) apply TAnn; try apply H with t_x k_sx k_tx; trivial.
   - (* TIf *) apply TIf with ps k (names_add x (union nms (binds (concatE g g'))));
     try apply H with t_x k_sx k_tx; 
@@ -137,54 +173,123 @@ Proof. apply ( judgments_mutind
     try assert (Cons y (self (TRefn TBool ps) (Bc false) Base) (concatE (Cons x s_x g) g') 
                   = concatE (Cons x s_x g) (Cons y (self (TRefn TBool ps) (Bc false) Base) g'))
       as Henv2 by reflexivity; try rewrite Henv2;     
+    apply H with g g' x s_x t_x k_sx k_tx in H11 as H';
+    try apply lem_typing_wf in H';  
     try apply H0 with y t_x k_sx k_tx; try apply H1 with y t_x k_sx k_tx;
+    try apply WFEBind with Base;
+    try apply lem_selfify_wf; try apply FTBC;
     try apply intersect_names_add_intro_r; 
     try apply not_elem_names_add_intro;
-    simpl; try split; auto. 
-  - (* TSub *) apply TSub with s k; try apply H with t_x k_sx k_tx;
-    try apply H0 with t_x k_sx k_tx; 
+    pose proof (lem_binds_concat (Cons x s_x g) g') as Hc;
+    try destruct Hc; try apply not_elem_names_add_intro; trivial;
+    try apply not_elem_subset with (union (binds (Cons x s_x g)) (binds g'));
+    try apply not_elem_union_intro;
+    try apply not_elem_names_add_intro; 
+    simpl; try discriminate; try split; auto;
+    inversion H'; assumption.
+  - (* TSub *) apply TSub with s k;
+    try apply H0 with t_x k_sx k_tx Star k; 
+    try apply lem_typing_wf with e;
+    try apply H with t_x k_sx k_tx;
     try apply lem_narrow_wf with t_x; trivial.
   - (* SBase *) try apply SBase with (names_add x (union nms (binds (concatE g g')))); 
+    apply lem_truncate_wfenv in H8 as H8'; inversion H8'; subst x0 t g0;
     intros; assert (Cons y (TRefn b PEmpty) (concatE (Cons x s_x g) g') 
                       = concatE (Cons x s_x g) (Cons y (TRefn b PEmpty) g'))
       as Henv by reflexivity; rewrite Henv;
     apply not_elem_names_add_elim in H; destruct H;
-    apply not_elem_union_elim in H9; destruct H9;
-    apply not_elem_concat_elim in H10; destruct H10.
+    apply not_elem_union_elim in H11; destruct H11;
+    apply not_elem_concat_elim in H12; destruct H12;
     apply INarrow with t_x k_sx k_tx; try apply i;
     try apply intersect_names_add_intro_r; try apply not_elem_names_add_intro;
     simpl; intuition.
-  - (* SFunc *) apply SFunc with (names_add x (union nms (binds (concatE g g'))));
-    try apply H with t_x k_sx k_tx; trivial; intros;
-    apply not_elem_names_add_elim in H1; destruct H1;
-    apply not_elem_union_elim in H11; destruct H11;
-    apply not_elem_concat_elim in H12; destruct H12;
+  - (* SFunc *) inversion H11; try inversion H1;
+    inversion H12; try inversion H19;
+    apply SFunc 
+      with (names_add x (union (union nms0 nms1) (union nms (binds (concatE g g')))));
+    try apply H with t_x k_sx k_tx k_x0 k_x; trivial; intros;
+    apply not_elem_names_add_elim in H26; destruct H26;
+    apply not_elem_union_elim in H27; destruct H27;
+    apply not_elem_union_elim in H27; destruct H27;
+    apply not_elem_union_elim in H28; destruct H28;
+    apply not_elem_concat_elim in H30; destruct H30;
     assert (Cons y s2 (concatE (Cons x s_x g) g') = concatE (Cons x s_x g) (Cons y s2 g'))
       as Henv by reflexivity; rewrite Henv;
-    apply H0 with t_x k_sx k_tx;
+    apply H0 with t_x k_sx k_tx k k0;
+    try apply WFEBind with k_x0; 
     try apply intersect_names_add_intro_r; 
-    try apply not_elem_names_add_intro; simpl; intuition.
+    try apply not_elem_names_add_intro; simpl; auto;
+    try apply lem_narrow_wf_top with s1;
+    try apply H with t_x k_sx k_tx k_x0 k_x; 
+    pose proof (lem_binds_concat (Cons x s_x g) g') as Hc;
+    try destruct Hc; trivial;
+    try apply not_elem_subset with (union (binds (Cons x s_x g)) (binds g'));
+    try apply not_elem_union_intro;
+    try apply not_elem_names_add_intro; 
+    try apply unique_concat;
+    try apply intersect_names_add_intro_l;
+    try split; simpl; auto.
   - (* SWitn *) apply SWitn with v_x;
     try apply H with t_x0 k_sx k_tx;
-    try apply H0 with t_x0 k_sx k_tx; trivial.
-  - (* SBind *) apply SBind with (names_add x (union nms (binds (concatE g g'))));
-    trivial; intros; apply not_elem_names_add_elim in H0; destruct H0;
-    apply not_elem_union_elim in H10; destruct H10;
-    apply not_elem_concat_elim in H11; destruct H11;
+    try apply H0 with t_x0 k_sx k_tx k_t k_t'; trivial.
+    inversion H12; try inversion H1;
+    pose proof (fresh_varT_not_elem nms (concatE (Cons x s_x g) g') t') as Hy; 
+    set (y := fresh_varT nms (concatE (Cons x s_x g) g') t') in Hy; 
+    destruct Hy as [Hyt' [_ [Hy Henv]]];
+    rewrite lem_tsubFV_unbindT with y v_x t';
+    try apply lem_subst_wf_top with t_x;
+    try apply H17; try apply WFKind; try apply H21;
+    try apply lem_typ_islc with g t_x0; 
+    try apply lem_typing_hasftype;
+    try apply H with t_x0 k_sx k_tx;
+    try apply unique_concat; 
+    try apply intersect_names_add_intro_l;
+    simpl; try split; trivial.
+  - (* SBind *) inversion H10; try inversion H0; subst t0 k g0; simpl;
+    apply SBind with (names_add x (union (union nms nms0) (binds (concatE g g'))));
+    trivial; intros; apply not_elem_names_add_elim in H12; destruct H12;
+    apply not_elem_union_elim in H13; destruct H13 as [H13 H19]; 
+    apply not_elem_union_elim in H13; destruct H13;
+    apply not_elem_concat_elim in H19; destruct H19;
     assert (Cons y t_x (concatE (Cons x s_x g) g') = concatE (Cons x s_x g) (Cons y t_x g'))
       as Henv by reflexivity; rewrite Henv;
-    apply H with t_x0 k_sx k_tx;
+    apply H with t_x0 k_sx k_tx k_t k_t';
+    try apply H16; destruct k_t; 
+    try apply WFKind; try apply H20;
+    try apply lem_weaken_wf_top;
+    try apply WFEBind with k_x;
     try apply intersect_names_add_intro_r; 
-    try apply not_elem_names_add_intro; simpl; intuition.
-  - (* SPoly *) apply SPoly with (names_add x (union nms (binds (concatE g g'))));
-    trivial; intros; apply not_elem_names_add_elim in H0; destruct H0;
-    apply not_elem_union_elim in H10; destruct H10;
-    apply not_elem_concat_elim in H11; destruct H11;
+    try apply not_elem_names_add_intro; 
+    pose proof (lem_binds_concat (Cons x s_x g) g') as Hbin;
+    try destruct Hbin; trivial;
+    try apply not_elem_subset with (union (binds (Cons x s_x g)) (binds g'));
+    try apply not_elem_union_intro;
+    try apply not_elem_names_add_intro; 
+    try apply unique_concat;
+    try apply intersect_names_add_intro_l; simpl; auto.
+  - (* SPoly *) inversion H10; try inversion H0;
+    inversion H11; try inversion H17;
+    apply SPoly 
+      with (names_add x (union (union nms0 nms1) (union nms (binds (concatE g g')))));
+    trivial; intros;
+    apply not_elem_names_add_elim in H23; destruct H23;
+    apply not_elem_union_elim in H24; destruct H24;
+    apply not_elem_union_elim in H24; destruct H24;
+    apply not_elem_union_elim in H25; destruct H25;
+    apply not_elem_concat_elim in H27; destruct H27;
     assert (ConsT a k (concatE (Cons x s_x g) g') = concatE (Cons x s_x g) (ConsT a k g'))
       as Henv by reflexivity; rewrite Henv;
-    apply H with t_x k_sx k_tx;
+    apply H with t_x k_sx k_tx k_t0 k_t1;
+    try apply WFEBindT;
     try apply intersect_names_add_intro_r; 
-    try apply not_elem_names_add_intro; simpl; intuition.
+    try apply not_elem_names_add_intro; 
+    pose proof (lem_binds_concat (Cons x s_x g) g') as Hbin;
+    try destruct Hbin; trivial;
+    try apply not_elem_subset with (union (binds (Cons x s_x g)) (binds g'));
+    try apply not_elem_union_intro;
+    try apply not_elem_names_add_intro; 
+    try apply unique_concat;
+    try apply intersect_names_add_intro_l; simpl; auto.
   Qed.
 
 Lemma lem_narrow_typ : 
@@ -193,21 +298,25 @@ Lemma lem_narrow_typ :
             -> unique g -> unique g'
             -> intersect (binds g) (binds g') = empty
             -> ~ (in_env x g) -> ~ (in_env x g') 
-            -> WFtype g s_x k_sx -> WFtype g t_x k_tx -> Subtype g s_x t_x -> WFEnv g
+            -> WFtype g s_x k_sx -> WFtype g t_x k_tx -> Subtype g s_x t_x 
+            -> WFEnv (concatE (Cons x s_x g) g')
             -> Hastype (concatE (Cons x s_x g) g') e t .
 Proof. intros; pose proof lem_narrow_typ'; destruct H9 as [Htyp Hsub];
   apply Htyp with (concatE (Cons x t_x g) g') t_x k_sx k_tx; trivial. Qed.
 
 Lemma lem_narrow_subtype :
-  forall (g g':env) (x:vname) (s_x t_x:type) (k_sx k_tx:kind) (t : type) (t' : type),
+  forall (g g':env) (x:vname) (s_x t_x:type) (k_sx k_tx:kind) (t t':type) (k_t k_t':kind),
     Subtype (concatE (Cons x t_x g) g') t t'
             -> unique g -> unique g'
             -> intersect (binds g) (binds g') = empty
             -> ~ (in_env x g) -> ~ (in_env x g') 
-            -> WFtype g s_x k_sx -> WFtype g t_x k_tx -> Subtype g s_x t_x -> WFEnv g
+            -> WFtype g s_x k_sx -> WFtype g t_x k_tx -> Subtype g s_x t_x
+            -> WFEnv (concatE (Cons x s_x g) g')
+            -> WFtype (concatE (Cons x s_x g) g') t  k_t
+            -> WFtype (concatE (Cons x s_x g) g') t' k_t'
             -> Subtype (concatE (Cons x s_x g) g') t t' .
-Proof. intros; pose proof lem_narrow_typ'; destruct H9 as [Htyp Hsub];
-  apply Hsub with (concatE (Cons x t_x g) g') t_x k_sx k_tx; trivial. Qed.
+Proof. intros; pose proof lem_narrow_typ'; destruct H11 as [Htyp Hsub].
+  apply Hsub with (concatE (Cons x t_x g) g') t_x k_sx k_tx k_t k_t'; trivial. Qed.
 
 Lemma lem_narrow_typ_top : 
   forall (g:env) (x:vname) (s_x t_x:type) (k_sx k_tx:kind) (e:expr) (t:type),
@@ -217,14 +326,18 @@ Lemma lem_narrow_typ_top :
             -> Hastype (Cons x s_x g) e t .
 Proof. intros; assert (Cons x s_x g = concatE (Cons x s_x g) Empty) by reflexivity;
   rewrite H6; apply lem_narrow_typ with t_x k_sx k_tx; 
-  try apply intersect_empty_r; simpl; intuition. Qed.
+  try apply intersect_empty_r; try apply WFEBind with k_sx;
+  simpl; intuition. Qed.
 
 Lemma lem_narrow_subtype_top :
-  forall (g:env) (x:vname) (s_x t_x:type) (k_sx k_tx:kind) (t : type) (t' : type),
+  forall (g:env) (x:vname) (s_x t_x:type) (k_sx k_tx:kind) (t t':type) (k_t k_t':kind),
     Subtype (Cons x t_x g) t t'
             -> unique g -> ~ (in_env x g) 
             -> WFtype g s_x k_sx -> WFtype g t_x k_tx -> Subtype g s_x t_x -> WFEnv g
-            -> Subtype (Cons x s_x g) t t' .
+            -> WFtype  (Cons x s_x g) t  k_t
+            -> WFtype  (Cons x s_x g) t' k_t'
+            -> Subtype (Cons x s_x g) t  t' .
 Proof. intros; assert (Cons x s_x g = concatE (Cons x s_x g) Empty) by reflexivity;
-  rewrite H6; apply lem_narrow_subtype with t_x k_sx k_tx; 
-  try apply intersect_empty_r; simpl; intuition. Qed.
+  rewrite H8; apply lem_narrow_subtype with t_x k_sx k_tx k_t k_t'; 
+  try apply intersect_empty_r; try apply WFEBind with k_sx;
+  simpl; intuition. Qed.
