coq-SystemRF-1.1/SystemRF/LemmasWeakenTypTV.v
@@ -1,10 +1,15 @@
 Require Import SystemRF.BasicDefinitions.
 Require Import SystemRF.Names.
 Require Import SystemRF.SystemFTyping.
+Require Import SystemRF.BasicPropsSubstitution.
 Require Import SystemRF.BasicPropsEnvironments.
 Require Import SystemRF.WellFormedness.
 Require Import SystemRF.Typing.
+Require Import SystemRF.LemmasWeakenWF.
 Require Import SystemRF.LemmasWeakenWFTV.
+Require Import SystemRF.LemmasWellFormedness.
+Require Import SystemRF.SubstitutionLemmaWF.
+Require Import SystemRF.LemmasTyping.
 Require Import SystemRF.LemmasWeakenTyp.
 
 (*-----------------------------------------------------------
@@ -15,26 +20,30 @@ Lemma lem_weaken_tv_typ' : ( forall (g'g : env) (e : expr) (t : type),
     Hastype g'g e t -> ( forall (g g':env) (a:vname) (k_a:kind),
         g'g = concatE g g' -> unique g -> unique g'
                            -> intersect (binds g) (binds g') = empty
-                           -> ~ (in_env a g) -> ~ (in_env a g') -> WFEnv g 
+                           -> ~ (in_env a g) -> ~ (in_env a g') -> WFEnv (concatE g g')
                            -> Hastype (concatE (ConsT a k_a g) g') e t ) ) /\ (
   forall (g'g : env) (t : type) (t' : type),
-    Subtype g'g t t' -> ( forall (g g':env) (a:vname) (k_a:kind),
+    Subtype g'g t t' -> ( forall (g g':env) (a:vname) (k_a k_t k_t':kind),
         g'g = concatE g g' -> unique g -> unique g'
                            -> intersect (binds g) (binds g') = empty
-                           -> ~ (in_env a g) -> ~ (in_env a g') -> WFEnv g 
+                           -> ~ (in_env a g) -> ~ (in_env a g') -> WFEnv (concatE g g') 
+                           -> WFtype (concatE g g') t  k_t
+                           -> WFtype (concatE g g') t' k_t'
                            -> Subtype (concatE (ConsT a k_a g) g') t t') ).
 Proof. apply ( judgments_mutind 
   (fun (g'g : env) (e : expr) (t : type) (p_e_t : Hastype g'g e t) => 
     forall (g g':env) (a:vname) (k_a:kind),
       g'g = concatE g g' -> unique g -> unique g'
                          -> intersect (binds g) (binds g') = empty
-                         -> ~ (in_env a g) -> ~ (in_env a g') -> WFEnv g
+                         -> ~ (in_env a g) -> ~ (in_env a g') -> WFEnv (concatE g g')
                          -> Hastype (concatE (ConsT a k_a g) g') e t )
   (fun (g'g : env) (t : type) (t' : type) (p_t_t' : Subtype g'g t t') => 
-    forall (g g':env) (a:vname) (k_a:kind),
+    forall (g g':env) (a:vname) (k_a k_t k_t':kind),
       g'g = concatE g g' -> unique g -> unique g'
                          -> intersect (binds g) (binds g') = empty
-                         -> ~ (in_env a g) -> ~ (in_env a g') -> WFEnv g 
+                         -> ~ (in_env a g) -> ~ (in_env a g') -> WFEnv (concatE g g') 
+                         -> WFtype (concatE g g') t  k_t
+                         -> WFtype (concatE g g') t' k_t'
                          -> Subtype (concatE (ConsT a k_a g) g') t t')  
                          );
   intro env; intros; subst env.
@@ -50,9 +59,13 @@ Proof. apply ( judgments_mutind
     apply not_elem_concat_elim in H8; destruct H8;
     assert (Cons y t_x (concatE (ConsT a k_a g) g') = concatE (ConsT a k_a g) (Cons y t_x g'))
       by reflexivity; rewrite H10;      
-    apply H; unfold in_env; simpl;
+    apply H; try apply WFEBind with k_x;
+    unfold in_env; simpl;
+    pose proof (lem_binds_concat g g'); destruct H11;
     try apply intersect_names_add_intro_r;
-    try apply not_elem_names_add_intro; intuition.    
+    try apply not_elem_names_add_intro; trivial;
+    try apply not_elem_subset with (union (binds g) (binds g'));
+    try apply not_elem_union_intro; auto.  
   - (* TApp *) apply TApp; apply H || apply H0; trivial.
   - (* TAbsT *) apply TAbsT with (names_add a (union nms (binds (concatE g g')))); intros;
     assert (ConsT a' k (concatE (ConsT a k_a g) g') = concatE (ConsT a k_a g) (ConsT a' k g'))
@@ -60,9 +73,13 @@ Proof. apply ( judgments_mutind
     apply not_elem_names_add_elim in H0; destruct H0; 
     apply not_elem_union_elim in H8; destruct H8;
     apply not_elem_concat_elim in H9; destruct H9;
-    apply H; unfold in_env; simpl;
+    apply H; try apply WFEBindT;
+    unfold in_env; simpl;
+    pose proof (lem_binds_concat g g'); destruct H11;
     try apply intersect_names_add_intro_r;
-    try apply not_elem_names_add_intro; intuition.
+    try apply not_elem_names_add_intro; trivial;
+    try apply not_elem_subset with (union (binds g) (binds g'));
+    try apply not_elem_union_intro; auto. 
   - (* TAppT *) apply TAppT with k; try apply H; try apply lem_weaken_tv_wf; trivial.
   - (* TLet *) apply TLet with t_x k (names_add a (union nms (binds (concatE g g'))));
     try apply H; try apply lem_weaken_tv_wf; trivial; intros;
@@ -71,9 +88,14 @@ Proof. apply ( judgments_mutind
     apply not_elem_names_add_elim in H1; destruct H1; 
     apply not_elem_union_elim in H9; destruct H9;
     apply not_elem_concat_elim in H10; destruct H10.
-    apply H0; unfold in_env; simpl;
+    apply H0; try apply WFEBind with Star;
+    unfold in_env; simpl;
+    try apply lem_typing_wf with e_x;
+    pose proof (lem_binds_concat g g'); destruct H12;
     try apply intersect_names_add_intro_r;
-    try apply not_elem_names_add_intro; intuition.
+    try apply not_elem_names_add_intro; trivial;
+    try apply not_elem_subset with (union (binds g) (binds g'));
+    try apply not_elem_union_intro; auto. 
   - (* TAnn *) apply TAnn; try apply H; trivial.
   - (* TIf *) apply TIf with ps k (names_add a (union nms (binds (concatE g g'))));
     try apply H; try apply lem_weaken_tv_wf; trivial; intros;
@@ -84,71 +106,134 @@ Proof. apply ( judgments_mutind
               = concatE (ConsT a k_a g) (Cons y (self (TRefn TBool ps) (Bc false) Base) g'))
       by reflexivity; try rewrite H10;
     apply H0 with y || apply H1 with y; 
+    try apply WFEBind with Base;
+    try apply lem_selfify_wf; try apply FTBC;
+    apply lem_typing_wf in h; 
     unfold in_env; simpl; try split;
     apply not_elem_names_add_elim in H2; destruct H2; 
     apply not_elem_union_elim in H11; destruct H11;
     apply not_elem_concat_elim in H12; destruct H12;
     try apply intersect_names_add_intro_r;
-    try apply not_elem_names_add_intro; intuition.
+    try apply not_elem_names_add_intro; trivial;
+    pose proof (lem_binds_concat g g'); try destruct H14; 
+    try apply not_elem_subset with (union (binds g) (binds g'));
+    try apply not_elem_union_intro;
+    inversion h; auto.
   - (* TSub *) apply TSub with s k; try apply H; try apply lem_weaken_tv_wf;
-    try apply H0; trivial.
+    try apply H0 with Star k; try apply lem_typing_wf with e; trivial.
   - (* SBase *) apply SBase with (names_add a (union nms (binds (concatE g g')))); intros;
     apply not_elem_names_add_elim in H; destruct H; 
-    apply not_elem_union_elim in H6; destruct H6;
-    apply not_elem_concat_elim in H7; destruct H7;
+    apply not_elem_union_elim in H8; destruct H8;
+    apply not_elem_concat_elim in H9; destruct H9;
     assert (Cons y (TRefn b PEmpty) (concatE (ConsT a k_a g) g') 
               = concatE (ConsT a k_a g) (Cons y (TRefn b PEmpty) g'))
-      by reflexivity; rewrite H9;
-    apply IWeakTV; unfold in_env; simpl;
+      by reflexivity; rewrite H11;
+    apply IWeakTV; try apply WFEBind with k_t;
+    unfold in_env; simpl;
     try apply intersect_names_add_intro_r;
-    try apply not_elem_names_add_intro; intuition.
-  - (* SFunc *) apply SFunc with (names_add a (union nms (binds (concatE g g'))));
-    try apply H; trivial; intros;
+    try apply not_elem_names_add_intro; trivial;
+    assert (WFtype (concatE g g') (TRefn b PEmpty) k_t) as Hwf
+      by (inversion H6; try inversion H12; try apply WFKind;
+          try (apply WFBase; apply H16 || apply H18); try apply H14;
+          try (apply WFVar; apply H16 || apply H20); try apply H18);
+    pose proof (lem_binds_concat g g'); try destruct H12;
+    try apply not_elem_subset with (union (binds g) (binds g'));
+    try apply not_elem_union_intro; auto.
+  - (* SFunc *) inversion H8; try inversion H1;
+    inversion H9; try inversion H16.
+    apply SFunc 
+      with (names_add a (union (union nms (union nms0 nms1)) (binds (concatE g g'))));
+    try apply H with k_x0 k_x; trivial; intros;
     assert (Cons y s2 (concatE (ConsT a k_a g) g') = concatE (ConsT a k_a g) (Cons y s2 g'))
-      by reflexivity; rewrite H8;
-    apply not_elem_names_add_elim in H1; destruct H1; 
-    apply not_elem_union_elim in H9; destruct H9;
-    apply not_elem_concat_elim in H10; destruct H10;
-    apply H0; unfold in_env; simpl;
+      by reflexivity; rewrite H24;
+    apply not_elem_names_add_elim in H23; destruct H23;  
+    apply not_elem_union_elim in H25; destruct H25; 
+    apply not_elem_union_elim in H25; destruct H25;
+    apply not_elem_union_elim in H27; destruct H27; 
+    apply not_elem_concat_elim in H26; destruct H26;
+    apply H0 with k k0; try apply WFEBind with k_x0;
+    unfold in_env; simpl; try apply H21;
+    try apply lem_narrow_wf_top with s1;
     try apply intersect_names_add_intro_r;
-    try apply not_elem_names_add_intro; intuition.
-  - (* SWitn *) apply SWitn with v_x; try apply H; try apply H0; trivial.
-  - (* SBind *) apply SBind with (names_add a (union nms (binds (concatE g g'))));
-    try apply i; intros;
+    try apply not_elem_names_add_intro; 
+    try apply not_elem_concat_intro;
+    try apply unique_concat; auto.
+  - (* SWitn *) apply SWitn with v_x; try apply H; 
+    try apply H0 with k_t k_t'; 
+    inversion H9; try inversion H1;
+    pose proof (fresh_varT_not_elem nms (concatE g g') t') as Hy; 
+    set (y := fresh_varT nms (concatE g g') t') in Hy; 
+    destruct Hy as [Hyt' [_ [Hy Henv]]];
+    try rewrite lem_tsubFV_unbindT with y v_x t';
+    try apply lem_subst_wf_top with t_x;
+    try apply WFKind;
+    try apply lem_typing_hasftype;
+    try apply unique_concat; auto. 
+  - (* SBind *) inversion H7; try inversion H0;
+    apply SBind with (names_add a (union (union nms nms0) (binds (concatE g g'))));
+    try apply i; intros y Hy;
     assert (Cons y t_x (concatE (ConsT a k_a g) g') = concatE (ConsT a k_a g) (Cons y t_x g'))
-      by reflexivity; rewrite H7;
-    apply not_elem_names_add_elim in H0; destruct H0; 
-    apply not_elem_union_elim in H8; destruct H8;
-    apply not_elem_concat_elim in H9; destruct H9;
-    apply H; unfold in_env; simpl;
+      as Henv by reflexivity; rewrite Henv; 
+    apply not_elem_names_add_elim in Hy; destruct Hy as [Hx Hy]; 
+    apply not_elem_union_elim in Hy; destruct Hy as [Hy Hyg];
+    apply not_elem_union_elim in Hy; destruct Hy;
+    apply not_elem_concat_elim in Hyg; destruct Hyg;
+    apply H with k_t k_t'; try apply WFEBind with k_x;
+    destruct k_t; try apply H13; try apply WFKind;
+    try apply H17; try apply lem_weaken_wf_top;
+    unfold in_env; simpl;
     try apply intersect_names_add_intro_r;
-    try apply not_elem_names_add_intro; intuition.
-  - (* SPoly *) apply SPoly with (names_add a (union nms (binds (concatE g g')))); intros;
+    try apply not_elem_names_add_intro; 
+    try apply not_elem_concat_intro; auto.
+  - (* SPoly *) inversion H7; try inversion H0;
+    inversion H8; try inversion H14;  
+    apply SPoly 
+      with (names_add a (union (union nms (union nms0 nms1)) (binds (concatE g g')))); 
+    intros;
     assert (ConsT a0 k (concatE (ConsT a k_a g) g') = concatE (ConsT a k_a g) (ConsT a0 k g'))
-      by reflexivity; rewrite H7;
-    apply not_elem_names_add_elim in H0; destruct H0; 
-    apply not_elem_union_elim in H8; destruct H8;
-    apply not_elem_concat_elim in H9; destruct H9;
-    apply H; unfold in_env; simpl;
+      by reflexivity; rewrite H21;
+    apply not_elem_names_add_elim in H20; destruct H20; 
+    apply not_elem_union_elim in H22; destruct H22;
+    apply not_elem_union_elim in H22; destruct H22;
+    apply not_elem_union_elim in H24; destruct H24;
+    apply not_elem_concat_elim in H23; destruct H23;
+    apply H with k_t0 k_t1; try apply WFEBindT;
+    unfold in_env; simpl;
     try apply intersect_names_add_intro_r;
-    try apply not_elem_names_add_intro; intuition.
+    try apply not_elem_names_add_intro; 
+    try apply not_elem_concat_intro;
+    try apply unique_concat; auto.
   Qed.
 
 Lemma lem_weaken_tv_typ : forall (g g':env) (e:expr) (t:type) (a:vname) (k_a:kind),
     Hastype (concatE g g') e t 
                           -> unique g -> unique g'
                           -> intersect (binds g) (binds g') = empty
-                          -> ~ (in_env a g) -> ~ (in_env a g') -> WFEnv g
+                          -> ~ (in_env a g) -> ~ (in_env a g') -> WFEnv (concatE g g')
                           -> Hastype (concatE (ConsT a k_a g) g') e t.
 Proof. intros; apply lem_weaken_tv_typ' with (concatE g g'); trivial. Qed.
 
-Lemma lem_weaken_tv_subtype : forall (g g':env) (t:type) (t':type) (a:vname) (k_a:kind),
+Lemma lem_weaken_tv_subtype : 
+  forall (g g':env) (t:type) (t':type) (a:vname) (k_a k_t k_t':kind),
     Subtype (concatE g g') t t' 
                           -> unique g -> unique g'
                           -> intersect (binds g) (binds g') = empty
-                          -> ~ (in_env a g) -> ~ (in_env a g') -> WFEnv g 
+                          -> ~ (in_env a g) -> ~ (in_env a g') -> WFEnv (concatE g g')
+                          -> WFtype (concatE g g') t  k_t
+                          -> WFtype (concatE g g') t' k_t'
                           -> Subtype (concatE (ConsT a k_a g) g') t t'.
-Proof. intros; apply lem_weaken_tv_typ' with (concatE g g'); trivial. Qed.
+Proof. intros; pose proof lem_weaken_tv_typ' as [_ Hweaken]; 
+  apply Hweaken with (concatE g g') k_t k_t'; trivial. Qed.
+
+Lemma lem_weaken_tv_subtype_top : 
+  forall (g:env) (t:type) (t':type) (a:vname) (k_a k_t k_t':kind),
+    Subtype g t t'  -> unique g -> ~ (in_env a g) -> WFEnv g
+                    -> WFtype g t k_t -> WFtype g t' k_t'
+                    -> Subtype (ConsT a k_a g) t t'.
+Proof. intros; assert (ConsT a k_a g = concatE (ConsT a k_a g) Empty) 
+    by reflexivity; rewrite H5; 
+  apply lem_weaken_tv_subtype with k_t k_t';
+  try apply intersect_empty_r; unfold unique; auto. Qed.  
 
 Lemma lem_weaken_many_typ : forall (g g':env) (e:expr) (t:type),
     Hastype g e t -> unique g -> unique g'
@@ -167,19 +252,18 @@ Proof. intros; induction g'; simpl; try assumption; inversion H3;
   try (apply not_elem_concat_intro; assumption);  
   intuition. Qed.
 
-Lemma lem_weaken_many_subtype : forall (g g':env) (t:type) (t':type),
+Lemma lem_weaken_many_subtype : 
+  forall (g g':env) (t:type) (t':type) (k_t k_t':kind),
     Subtype g t t' -> unique g -> unique g'
                    -> intersect (binds g) (binds g') = empty   
                    -> WFEnv (concatE g g')
+                   -> WFtype g t  k_t
+                   -> WFtype g t' k_t'
                    -> Subtype (concatE g g') t t'.
 Proof. intros; induction g'; simpl; try assumption;
   inversion H3; simpl in H1; destruct H1;
   simpl in H2; apply intersect_names_add_elim_r in H2; destruct H2;
-  apply IHg' in H2 as H'; try assumption;
-  apply lem_weaken_subtype with (concatE g g') Empty t t' x t0 in H'
-    || apply lem_weaken_tv_subtype with (concatE g g') Empty t t' a k in H';
-  simpl in H'; unfold in_env; simpl; 
-  try (apply intersect_empty_r);
-  try (apply unique_concat);
-  try (apply not_elem_concat_intro; assumption);  
-  intuition. Qed.
+  apply lem_weaken_subtype_top with k_t k_t'
+    || apply lem_weaken_tv_subtype_top with k_t k_t';
+  try apply IHg'; try apply lem_weaken_many_wf;
+  try apply unique_concat; trivial. Qed.
