coq-SystemRF-1.1/SystemRF/SubstitutionLemmaTypTV.v
@@ -4,14 +4,17 @@ Require Import SystemRF.BasicDefinitions.
 Require Import SystemRF.Names.
 Require Import SystemRF.LocalClosure.
 Require Import SystemRF.Strengthenings.
+Require Import SystemRF.SystemFWellFormedness.
 Require Import SystemRF.SystemFTyping.
 Require Import SystemRF.BasicPropsSubstitution.
 Require Import SystemRF.BasicPropsEnvironments.
 Require Import SystemRF.WellFormedness.
 Require Import SystemRF.BasicPropsWellFormedness.
 Require Import SystemRF.Typing.
+Require Import SystemRF.LemmasWeakenWF.
 Require Import SystemRF.LemmasWeakenWFTV.
 Require Import SystemRF.LemmasWellFormedness.
+Require Import SystemRF.SubstitutionLemmaWF.
 Require Import SystemRF.SubstitutionLemmaWFTV.
 Require Import SystemRF.LemmasTyping.
 Require Import SystemRF.LemmasWeakenTypTV.
@@ -25,15 +28,18 @@ Lemma lem_subst_tv_typ' : ( forall (g'ag : env) (e : expr) (t : type),
             -> unique g -> unique g'
             -> intersect (binds g) (binds g') = empty
             -> ~ (in_env a g) -> ~ (in_env a g') 
-            -> isMono t_a -> noExists t_a -> WFtype g t_a k_a -> WFEnv g
+            -> isMono t_a -> noExists t_a -> WFtype g t_a k_a -> WFEnv (concatE (ConsT a k_a g) g')
             -> Hastype (concatE g (esubFTV a t_a g')) (subFTV a t_a e) (tsubFTV a t_a t ) )) /\ (
   forall (g'ag : env) (t : type) (t' : type),
-    Subtype g'ag t t' -> ( forall (g g':env) (a:vname) (t_a:type) (k_a:kind),
+    Subtype g'ag t t' -> ( forall (g g':env) (a:vname) (t_a:type) (k_a k_t k_t':kind),
     g'ag = concatE (ConsT a k_a g) g'  
         -> unique g -> unique g'
         -> intersect (binds g) (binds g') = empty
         -> ~ (in_env a g) -> ~ (in_env a g') 
-        -> isMono t_a -> noExists t_a -> WFtype g t_a k_a -> WFEnv g
+        -> isMono t_a -> noExists t_a -> WFtype g t_a k_a
+        -> WFEnv (concatE (ConsT a k_a g) g')
+        -> WFtype (concatE (ConsT a k_a g) g') t  k_t
+        -> WFtype (concatE (ConsT a k_a g) g') t' k_t'
         -> Subtype (concatE g (esubFTV a t_a g')) (tsubFTV a t_a t) (tsubFTV a t_a t') )).
 Proof. apply ( judgments_mutind 
   (fun (g'ag : env) (e : expr) (t : type) (p_e_t : Hastype g'ag e t) => 
@@ -42,20 +48,24 @@ Proof. apply ( judgments_mutind
             -> unique g -> unique g'
             -> intersect (binds g) (binds g') = empty
             -> ~ (in_env a g) -> ~ (in_env a g') 
-            -> isMono t_a -> noExists t_a -> WFtype g t_a k_a -> WFEnv g
+            -> isMono t_a -> noExists t_a -> WFtype g t_a k_a -> WFEnv (concatE (ConsT a k_a g) g')
             -> Hastype (concatE g (esubFTV a t_a g')) (subFTV a t_a e) (tsubFTV a t_a t ) )
   (fun (g'ag : env) (t : type) (t' : type) (p_t_t' : Subtype g'ag t t') => 
-    forall (g g':env) (a:vname) (t_a:type) (k_a:kind),
+    forall (g g':env) (a:vname) (t_a:type) (k_a k_t k_t':kind),
       g'ag = concatE (ConsT a k_a g) g'  
         -> unique g -> unique g'
         -> intersect (binds g) (binds g') = empty
         -> ~ (in_env a g) -> ~ (in_env a g') 
-        -> isMono t_a -> noExists t_a -> WFtype g t_a k_a -> WFEnv g
+        -> isMono t_a -> noExists t_a -> WFtype g t_a k_a 
+        -> WFEnv (concatE (ConsT a k_a g) g')
+        -> WFtype (concatE (ConsT a k_a g) g') t  k_t
+        -> WFtype (concatE (ConsT a k_a g) g') t' k_t'
         -> Subtype (concatE g (esubFTV a t_a g')) (tsubFTV a t_a t) (tsubFTV a t_a t') ) );
   intro env; intros; subst env.
   - (* TBC *) rewrite lem_tsubFTV_tybc; try apply TBC; assumption.
   - (* TIC *) rewrite lem_tsubFTV_tyic; try apply TIC; assumption.
-  - (* TVar *) apply lem_boundin_concat in b; simpl in b; simpl; destruct k.
+  - (* TVar *) apply lem_boundin_concat in b; simpl in b; simpl; destruct k;
+    apply lem_truncate_wfenv in H8 as H8'; inversion H8'; subst a0 k g0.
     * (* Base *) apply TSub with (self (tsubFTV a t_a t) (FV x) Base) Base;
       try apply TVar; try apply lem_boundin_concat; 
       try ( apply lem_subst_tv_wf' with k_a; try apply lem_selfify_wf);
@@ -64,10 +74,10 @@ Proof. apply ( judgments_mutind
       try apply lem_wftype_islct with (concatE (ConsT a k_a g) g') Base;
       try apply FTVar; try apply boundin_erase_env; try rewrite lem_boundin_concat;
       destruct b;
-      try apply (boundin_wfenv_wftype x t g H) in H8 as p_g_t;
+      try apply (boundin_wfenv_wftype x t g H) in H10 as p_g_t;
       try ( left; pose proof lem_subFTV_notin; destruct H9; destruct p; rewrite e0;
             try apply H; apply lem_free_bound_in_env with g Star );
-      try ( right; apply lem_boundin_esubFTV ); simpl; intuition.
+      try ( right; apply lem_boundin_esubFTV ); simpl; auto.
     * (* Star *) rewrite lem_self_star; 
       rewrite <- lem_self_star with (tsubFTV a t_a t) (FV x); apply TVar;
       try apply lem_boundin_concat; destruct b; 
@@ -78,35 +88,47 @@ Proof. apply ( judgments_mutind
       try (apply boundin_wfenv_wftype with x; assumption); assumption.
   - (* TPrm *) rewrite lem_tsubFTV_ty; simpl; try apply TPrm; assumption.
   - (* TAbs *) simpl; apply TAbs with k_x (names_add a (union nms (binds (concatE g g'))));
+    apply lem_truncate_wfenv in H9 as H9'; inversion H9'; subst a0 k g0;
     try apply lem_subst_tv_wf' with k_a; try assumption; intros;
     apply not_elem_names_add_elim in H0; destruct H0;
     apply not_elem_union_elim in H10; destruct H10;
-    apply not_elem_concat_elim in H11; destruct H11;
+    apply not_elem_concat_elim in H12; destruct H12;
     assert (Cons y (tsubFTV a t_a t_x) (concatE g (esubFTV a t_a g')) 
             = concatE g (esubFTV a t_a (Cons y t_x g')))
-      by reflexivity; rewrite H13;
+      by reflexivity; rewrite H15;
     rewrite <- lem_commute_subFTV_unbind;
     try rewrite <- lem_commute_tsubFTV_unbindT;
     try apply H with k_a;
+    try apply WFEBind with k_x; 
     try apply intersect_names_add_intro_r;  
     try apply lem_wftype_islct with g k_a;
-    unfold in_env; try apply not_elem_names_add_intro;
-    simpl; intuition.
+    pose proof (lem_binds_concat (ConsT a k_a g) g');
+    destruct H16; try apply not_elem_names_add_intro; trivial;
+    try apply not_elem_subset with (union (binds (ConsT a k_a g)) (binds g'));
+    try apply not_elem_union_intro;
+    try apply not_elem_names_add_intro;
+    simpl; auto.
   - (* TApp *) simpl; apply TApp; simpl in H; 
     apply H with k_a || apply H0 with k_a; trivial.
   - (* TAbsT *) simpl; apply TAbsT with (names_add a (union nms (binds (concatE g g'))));
+    apply lem_truncate_wfenv in H9 as H9'; inversion H9'; subst a0 k0 g0;
     intros; apply not_elem_names_add_elim in H0; destruct H0;
     apply not_elem_union_elim in H10; destruct H10;
-    apply not_elem_concat_elim in H11; destruct H11;
+    apply not_elem_concat_elim in H12; destruct H12;
     assert (ConsT a' k (concatE g (esubFTV a t_a g')) = concatE g (esubFTV a t_a (ConsT a' k g')))
-      by reflexivity; rewrite H13;
+      by reflexivity; rewrite H15;
     try rewrite <- lem_commute_subFTV_unbind_tv;
     try rewrite <- lem_commute_tsubFTV_unbind_tvT;
-    try apply H with k_a;
+    try apply H with k_a; try apply WFEBindT;
     try apply intersect_names_add_intro_r;
     try apply lem_wftype_islct with g k_a;
-    unfold in_env; try apply not_elem_names_add_intro; simpl; intuition.
+    pose proof (lem_binds_concat (ConsT a k_a g) g');
+    destruct H16; try apply not_elem_names_add_intro; trivial;
+    try apply not_elem_subset with (union (binds (ConsT a k_a g)) (binds g'));
+    try apply not_elem_union_intro;
+    try apply not_elem_names_add_intro; simpl; auto.
   - (* TAppT *) rewrite lem_commute_tsubFTV_tsubBTV; simpl;
+    apply lem_truncate_wfenv in H9 as H9'; inversion H9'; subst a0 k0 g0;
     try apply TAppT with k; simpl in H;
     try apply H with k_a;
     try apply lemma_tsubFTV_isMono;
@@ -115,48 +137,69 @@ Proof. apply ( judgments_mutind
     try apply lem_wftype_islct with g k_a; trivial.
   - (* TLet *) simpl; apply TLet with (tsubFTV a t_a t_x) k
                   (names_add a (union nms (binds (concatE g g'))));
+    apply lem_truncate_wfenv in H10 as H10'; inversion H10'; subst a0 k0 g0;
     try apply lem_subst_tv_wf' with k_a;
     try apply H with k_a; trivial; intros;
     apply not_elem_names_add_elim in H1; destruct H1;
     apply not_elem_union_elim in H11; destruct H11;
-    apply not_elem_concat_elim in H12; destruct H12;
+    apply not_elem_concat_elim in H13; destruct H13;
     assert (Cons y (tsubFTV a t_a t_x) (concatE g (esubFTV a t_a g')) 
             = concatE g (esubFTV a t_a (Cons y t_x g')))
-      by reflexivity; rewrite H14;
+      by reflexivity; rewrite H16;
     rewrite <- lem_commute_subFTV_unbind;
     try rewrite <- lem_commute_tsubFTV_unbindT;
-    try apply H0 with k_a;
+    try apply H0 with k_a; try apply WFEBind with Star;
     try apply intersect_names_add_intro_r;
     try apply lem_wftype_islct with g k_a;
-    try apply not_elem_names_add_intro; simpl; auto.
+    try apply not_elem_names_add_intro;
+    pose proof (lem_binds_concat (ConsT a k_a g) g');
+    destruct H17; trivial;
+    try apply not_elem_subset with (union (binds (ConsT a k_a g)) (binds g'));
+    try apply not_elem_union_intro;
+    try apply not_elem_names_add_intro; 
+    try apply lem_typing_wf with e_x;  
+    simpl; auto.
   - (* TAnn *) simpl; apply TAnn; try apply lemma_tsubFTV_noExists;
     try apply H with k_a; trivial.
   - (* TIf *) simpl; apply TIf with (psubFTV a t_a ps) k 
                                     (names_add a (union nms (binds (concatE g g'))));
+    apply lem_truncate_wfenv in H11 as H11'; inversion H11'; subst a0 k0 g0;
     simpl in H; try apply H with k_a;
-    try apply lem_subst_tv_wf with k_a;
-    try apply lem_typing_hasftype; intros;
-    try apply not_elem_names_add_elim in H2; try destruct H2;
-    try apply not_elem_union_elim in H12; try destruct H12; 
-    try apply not_elem_concat_elim in H13; try destruct H13;     
+    try apply lem_subst_tv_wf with k_a; 
+    try apply lem_erase_env_wfenv; trivial; intros;
+    apply not_elem_names_add_elim in H2; destruct H2;
+    apply not_elem_union_elim in H12; destruct H12; 
+    apply not_elem_concat_elim in H14; destruct H14;     
     try assert (Cons y (self (TRefn TBool (psubFTV a t_a ps)) (Bc true) Base) 
                        (concatE g (esubFTV a t_a g')) 
             = concatE g (esubFTV a t_a (Cons y (self (TRefn TBool ps) (Bc true) Base) g')))
-      by reflexivity; try rewrite H15; 
+      by reflexivity; try rewrite H17; 
     try assert (Cons y (self (TRefn TBool (psubFTV a t_a ps)) (Bc false) Base)  
                        (concatE g (esubFTV a t_a g')) 
             = concatE g (esubFTV a t_a (Cons y (self (TRefn TBool ps) (Bc false) Base) g')))
-      by reflexivity; try rewrite H16; 
+      by reflexivity; try rewrite H18; 
     try apply H0 with y k_a; try apply H1 with y k_a; 
-    try apply lem_erase_env_wfenv;
+    try apply WFEBind with Base; fold concatE;
+    try apply lem_selfify_wf; try apply FTBC;
     try apply not_elem_names_add_intro;
     try apply intersect_names_add_intro_r;
-    simpl; try split; auto. 
+    pose proof (lem_binds_concat (ConsT a k_a g) g');
+    try destruct H19; trivial; 
+    try apply not_elem_subset with (union (binds (ConsT a k_a g)) (binds g'));
+    try apply not_elem_union_intro;
+    try apply not_elem_names_add_intro; 
+    simpl; try discriminate; try split; auto;
+    apply lem_typing_wf in h; try apply H10; 
+    inversion h; trivial.
   - (* TSub *) apply TSub with (tsubFTV a t_a s) k; 
+    apply lem_truncate_wfenv in H10 as H10'; inversion H10'; subst a0 k0 g0;
     try apply H with k_a; try apply lem_subst_tv_wf' with k_a;
-    try apply H0 with k_a; trivial.
-  - (* SBase *) destruct b eqn:B; try destruct (Nat.eqb a a0) eqn:A; 
-    simpl; try rewrite A;
+    try apply H0 with k_a Star k; 
+    try apply lem_typing_wf with e; trivial.
+  - (* SBase *) 
+    apply lem_truncate_wfenv in H8 as H8'; inversion H8'; subst a0 k g0;
+    destruct b eqn:B; try destruct (Nat.eqb a a0) eqn:A; 
+    simpl; try rewrite A; 
     try ( apply SBase with (names_add a (union nms (binds (concatE g g'))));
           intros; repeat rewrite <- lem_commute_psubFTV_unbindP; try rewrite <- B;
           assert ( Cons y (TRefn b PEmpty) (concatE g (esubFTV a t_a g'))
@@ -165,8 +208,8 @@ Proof. apply ( judgments_mutind
           try rewrite Henv;
           try apply ISubTV with k_a; try (rewrite B; apply i);
           apply not_elem_names_add_elim in H; destruct H;
-          apply not_elem_union_elim in H9; destruct H9;
-          apply not_elem_concat_elim in H10; destruct H10;
+          apply not_elem_union_elim in H11; destruct H11;
+          apply not_elem_concat_elim in H13; destruct H13;
           try apply lem_wftype_islct with g k_a;
           try apply not_elem_names_add_intro;
           try apply intersect_names_add_intro_r;
@@ -179,8 +222,8 @@ Proof. apply ( judgments_mutind
           trivial).
     apply SBase with (names_add a (union nms (binds (concatE g g')))); intros;
     apply not_elem_names_add_elim in H; destruct H;
-    apply not_elem_union_elim in H9; destruct H9;
-    apply not_elem_concat_elim in H10; destruct H10;
+    apply not_elem_union_elim in H11; destruct H11;
+    apply not_elem_concat_elim in H13; destruct H13;
     repeat rewrite lem_unbindP_strengthen; apply IStren;
     try apply not_elem_concat_intro; try rewrite esubFTV_binds; trivial;
     repeat rewrite <- lem_commute_psubFTV_unbindP; try repeat rewrite <- TA;
@@ -194,50 +237,105 @@ Proof. apply ( judgments_mutind
     try rewrite TA; try apply lem_wftype_islct with g k_a;
     try apply intersect_names_add_intro_r; 
     try apply not_elem_names_add_intro; intuition.
-  - (* SFunc *) simpl; apply SFunc with (names_add a (union nms (binds (concatE g g'))));
-    try apply H with k_a; trivial; intros;
-    apply not_elem_names_add_elim in H1; destruct H1;
-    apply not_elem_union_elim in H11; destruct H11;
-    apply not_elem_concat_elim in H12; destruct H12;
+  - (* SFunc *)
+    apply lem_truncate_wfenv in H10 as H10'; inversion H10'; subst a0 k g0;
+    inversion H11; try inversion H1;
+    inversion H12; try inversion H21;
+    simpl; apply SFunc 
+      with (names_add a (union (union nms0 nms1) (union nms (binds (concatE g g')))));
+    try apply H with k_a k_x0 k_x; trivial; intros;
+    apply not_elem_names_add_elim in H28; destruct H28;
+    apply not_elem_union_elim in H29; destruct H29;
+    apply not_elem_union_elim in H29; destruct H29;
+    apply not_elem_union_elim in H30; destruct H30;
+    apply not_elem_concat_elim in H32; destruct H32;
     repeat rewrite <- lem_commute_tsubFTV_unbindT;
     assert (Cons y (tsubFTV a t_a s2) (concatE g (esubFTV a t_a g')) 
             = concatE g (esubFTV a t_a (Cons y s2 g')))
-      by reflexivity; try rewrite H14;
-    try apply H0 with k_a;
+      by reflexivity; try rewrite H34;
+    try apply H0 with k_a k k0;    
+    try apply H26; try apply H19 in H29 as H19';
+    try apply lem_narrow_wf_top with s1; fold concatE;
     try apply intersect_names_add_intro_r;  
     try apply lem_wftype_islct with g k_a;
-    try apply not_elem_names_add_intro; simpl; intuition.
+    try apply not_elem_names_add_intro; 
+    try apply WFEBind with k_x0;
+    pose proof (lem_binds_concat (ConsT a k_a g) g');
+    try destruct H35; try apply not_elem_names_add_intro; trivial;
+    try apply not_elem_subset with (union (binds (ConsT a k_a g)) (binds g'));
+    try apply not_elem_union_intro;
+    try apply not_elem_names_add_intro; 
+    try apply unique_concat;
+    try apply intersect_names_add_intro_l;
+    try split; simpl; auto. 
   - (* SWitn *) simpl; apply SWitn with (subFTV a t_a v_x);
+    apply lem_truncate_wfenv in H10 as H10'; inversion H10'; subst a0 k g0;
     try apply lem_subFTV_value; try apply H with k_a;
     try rewrite <- lem_commute_tsubFTV_tsubBV;
-    try apply H0 with k_a; try apply lem_wftype_islct with g k_a;    
-    trivial.
-  - (* SBind *) simpl; apply SBind with (names_add a (union nms (binds (concatE g g'))));
+    try apply H0 with k_a k_t k_t';
+    inversion H12; try inversion H1;
+    pose proof (fresh_varT_not_elem nms (concatE (ConsT a k_a g) g') t') as Hy; 
+    set (y := fresh_varT nms (concatE (ConsT a k_a g) g') t') in Hy; 
+    destruct Hy as [Hyt' [_ [Hy Henv]]];
+    try rewrite lem_tsubFV_unbindT with y v_x t'; 
+    try apply lem_subst_wf_top with t_x;
+    try apply H19; try apply WFKind; try apply H23;
+    try apply lem_wftype_islct with g k_a;    
+    try apply lem_typing_hasftype;
+    try apply unique_concat; 
+    try apply intersect_names_add_intro_l;
+    simpl; try split; trivial.
+  - (* SBind *) 
+    apply lem_truncate_wfenv in H9 as H9'; inversion H9'; subst a0 k g0;
+    inversion H10; try inversion H0; subst t0 k g0; simpl; 
+    apply SBind with (names_add a (union (union nms nms0) (binds (concatE g g'))));
     try apply lem_islc_at_subFTV; try apply (lem_wftype_islct g t_a) with k_a;
-    trivial; intros;
-    apply not_elem_names_add_elim in H0; destruct H0;
-    apply not_elem_union_elim in H10; destruct H10;
-    apply not_elem_concat_elim in H11; destruct H11;
-    try rewrite <- lem_commute_tsubFTV_unbindT;
+    trivial; intros y Hy;
+    apply not_elem_names_add_elim in Hy; destruct Hy;
+    apply not_elem_union_elim in H14; destruct H14 as [H14 Hyg];
+    apply not_elem_union_elim in H14; destruct H14;
+    apply not_elem_concat_elim in Hyg; destruct Hyg;
+    rewrite <- lem_commute_tsubFTV_unbindT;
     assert (Cons y (tsubFTV a t_a t_x) (concatE g (esubFTV a t_a g')) 
-            = concatE g (esubFTV a t_a (Cons y t_x g')))
-      by reflexivity; try rewrite H13;
-    try apply H with k_a;
+            = concatE g (esubFTV a t_a (Cons y t_x g'))) as Henv
+      by reflexivity; try rewrite Henv;
+    try apply H with k_a k_t k_t';
+    try apply H18; destruct k_t; try apply WFKind; 
+    try apply H22; try apply lem_weaken_wf_top;
+    try apply WFEBind with k_x;
     try apply intersect_names_add_intro_r;  
     try apply lem_wftype_islct with g k_a;
-    try apply not_elem_names_add_intro; simpl; intuition.
-  - (* SPoly *) simpl; apply SPoly with (names_add a (union nms (binds (concatE g g'))));
-    intros; apply not_elem_names_add_elim in H0; destruct H0;
-    apply not_elem_union_elim in H10; destruct H10;
-    apply not_elem_concat_elim in H11; destruct H11;
+    try apply not_elem_names_add_intro; 
+    pose proof (lem_binds_concat (ConsT a k_a g) g') as Hbin;
+    try destruct Hbin; trivial;
+    try apply not_elem_subset with (union (binds (ConsT a k_a g)) (binds g'));
+    try apply not_elem_union_intro;
+    try apply not_elem_names_add_intro; simpl; auto. 
+  - (* SPoly *) 
+    apply lem_truncate_wfenv in H9 as H9'; inversion H9'; subst a0 k0 g0;
+    inversion H10; try inversion H0;
+    inversion H11; try inversion H19; simpl; 
+    apply SPoly with (names_add a (union (union nms0 nms1) (union nms (binds (concatE g g')))));
+    intros; apply not_elem_names_add_elim in H25; destruct H25;
+    apply not_elem_union_elim in H26; destruct H26;
+    apply not_elem_union_elim in H26; destruct H26;
+    apply not_elem_union_elim in H27; destruct H27;
+    apply not_elem_concat_elim in H29; destruct H29;
     repeat rewrite <- lem_commute_tsubFTV_unbind_tvT;
     assert (ConsT a0 k (concatE g (esubFTV a t_a g')) 
               = concatE g (esubFTV a t_a (ConsT a0 k g')))
-        by reflexivity; try rewrite H13;
-    try apply H with k_a;
-    try apply lem_wftype_islct with g k_a; 
+        by reflexivity; try rewrite H31;
+    try apply H with k_a k_t0 k_t1;
+    try apply lem_wftype_islct with g k_a;
+    try apply WFEBindT;
     try apply not_elem_names_add_intro;
-    try apply intersect_names_add_intro_r; simpl; try split; intuition.
+    try apply intersect_names_add_intro_r; 
+    pose proof (lem_binds_concat (ConsT a k_a g) g') as Hbin;
+    try destruct Hbin; trivial;
+    try apply not_elem_subset with (union (binds (ConsT a k_a g)) (binds g'));
+    try apply not_elem_union_intro;
+    try apply not_elem_names_add_intro; 
+    simpl; try split; auto.  
   Qed.
 
 Lemma lem_subst_tv_typ : forall (g g':env) (a:vname) (t_a:type) (k_a:kind) (e:expr) (t:type),
@@ -245,7 +343,8 @@ Lemma lem_subst_tv_typ : forall (g g':env) (a:vname) (t_a:type) (k_a:kind) (e:ex
             -> unique g -> unique g'
             -> intersect (binds g) (binds g') = empty
             -> ~ (in_env a g) -> ~ (in_env a g') 
-            -> isMono t_a -> noExists t_a -> WFtype g t_a k_a -> WFEnv g
+            -> isMono t_a -> noExists t_a -> WFtype g t_a k_a 
+            -> WFEnv (concatE (ConsT a k_a g) g')
             -> Hastype (concatE g (esubFTV a t_a g')) (subFTV a t_a e) (tsubFTV a t_a t ).
 Proof. intros; pose proof lem_subst_tv_typ'; destruct H9 as [Htyp Hsub];
   apply Htyp with (concatE (ConsT a k_a g) g') k_a; trivial. Qed.
@@ -257,23 +356,31 @@ Lemma lem_subst_tv_typ_top : forall (g:env) (a:vname) (t_a:type) (k_a:kind) (e:e
             -> Hastype g (subFTV a t_a e) (tsubFTV a t_a t).
 Proof. intros; assert (g = concatE g (esubFTV a t_a Empty)) by reflexivity;
   rewrite H6; apply lem_subst_tv_typ with k_a; try apply intersect_empty_r; 
-  unfold unique; intuition. Qed.
+  try apply WFEBindT; unfold unique; auto. Qed.
 
-Lemma lem_subst_tv_subtype : forall (g g':env) (a:vname) (t_a:type) (k_a:kind) (t t':type),
+Lemma lem_subst_tv_subtype : 
+  forall (g g':env) (a:vname) (t_a:type) (k_a:kind) (t t':type) (k_t k_t':kind),
         Subtype (concatE (ConsT a k_a g) g') t t' 
             -> unique g -> unique g'
             -> intersect (binds g) (binds g') = empty
             -> ~ (in_env a g) -> ~ (in_env a g') 
-            -> isMono t_a -> noExists t_a -> WFtype g t_a k_a -> WFEnv g
+            -> isMono t_a -> noExists t_a -> WFtype g t_a k_a 
+            -> WFEnv (concatE (ConsT a k_a g) g')
+            -> WFtype (concatE (ConsT a k_a g) g') t  k_t
+            -> WFtype (concatE (ConsT a k_a g) g') t' k_t'
             -> Subtype (concatE g (esubFTV a t_a g')) (tsubFTV a t_a t) (tsubFTV a t_a t').
-Proof. intros; pose proof lem_subst_tv_typ'; destruct H9 as [Htyp Hsub];
-  apply Hsub with (concatE (ConsT a k_a g) g') k_a; trivial. Qed.
+Proof. intros; pose proof lem_subst_tv_typ'; destruct H11 as [Htyp Hsub];
+  apply Hsub with (concatE (ConsT a k_a g) g') k_a k_t k_t'; trivial. Qed.
 
-Lemma lem_subst_tv_subtype_top : forall (g:env) (a:vname) (t_a:type) (k_a:kind) (t t':type),
+Lemma lem_subst_tv_subtype_top : 
+  forall (g:env) (a:vname) (t_a:type) (k_a:kind) (t t':type) (k_t k_t':kind),
         Subtype (ConsT a k_a g) t t' 
             -> unique g -> ~ (in_env a g) 
             -> isMono t_a -> noExists t_a -> WFtype g t_a k_a -> WFEnv g
+            -> WFtype (ConsT a k_a g) t  k_t
+            -> WFtype (ConsT a k_a g) t' k_t'
             -> Subtype g (tsubFTV a t_a t) (tsubFTV a t_a t').
 Proof. intros; assert (g = concatE g (esubFTV a t_a Empty)) by reflexivity;
-  rewrite H6; apply lem_subst_tv_subtype with k_a; try apply intersect_empty_r; 
+  rewrite H8; apply lem_subst_tv_subtype with k_a k_t k_t'; 
+  try apply intersect_empty_r; try apply WFEBindT;
   unfold unique; intuition. Qed.
