coq-SystemRF-1.1/compile.sh
@@ -41,10 +41,6 @@ echo "Checking LemmasWeakenWF.v ..."
 coqc -R SystemRF SystemRF SystemRF/LemmasWeakenWF.v
 echo "Checking LemmasWeakenWFTV.v ..."
 coqc -R SystemRF SystemRF SystemRF/LemmasWeakenWFTV.v
-echo "Checking LemmasWeakenTyp.v ..."
-coqc -R SystemRF SystemRF SystemRF/LemmasWeakenTyp.v
-echo "Checking LemmasWeakenTypTV.v ..."
-coqc -R SystemRF SystemRF SystemRF/LemmasWeakenTypTV.v
 echo "Checking LemmasWellFormedness.v ..."
 coqc -R SystemRF SystemRF SystemRF/LemmasWellFormedness.v
 echo "Checking PrimitivesWFType.v ..."
@@ -55,6 +51,10 @@ echo "Checking SubstitutionLemmaWFTV.v ..."
 coqc -R SystemRF SystemRF SystemRF/SubstitutionLemmaWFTV.v
 echo "Checking LemmasTyping.v ..."
 coqc -R SystemRF SystemRF SystemRF/LemmasTyping.v
+echo "Checking LemmasWeakenTyp.v ..."
+coqc -R SystemRF SystemRF SystemRF/LemmasWeakenTyp.v
+echo "Checking LemmasWeakenTypTV.v ..."
+coqc -R SystemRF SystemRF SystemRF/LemmasWeakenTypTV.v
 echo "Checking LemmasSubtyping.v ..."
 coqc -R SystemRF SystemRF SystemRF/LemmasSubtyping.v
 echo "Checking LemmasExactness.v ..."
